firmware/IncrementWait/CavaIncrementDevice.v
@@ -1,9 +1,13 @@
 From Coq Require Import
+     Lists.List
      ZArith.ZArith.
+
+Import ListNotations.
 
 From Cava Require Import
      Expr
      Primitives
+     Semantics
      Types.
 
 Import ExprNotations.
@@ -18,6 +22,8 @@ Section Var.
   (* Things that should probably be in cava *)
   Section Cava.
     Definition True := Constant (true: denote_type Bit).
+
+    Definition circuit_state {i s o} (c : Circuit s i o) := denote_type s.
   End Cava.
 
   Definition incr
@@ -63,34 +69,43 @@ Section Var.
        }}.
 End Var.
 
-Definition incr_device_step:
+Example sample_trace :=
+  Eval compute in simulate incr
+                           [ (false,   (false, (111%N, (111%N, tt)))) (* no action *)
+                             ; (false, (true,  (  0%N, ( 15%N, tt)))) (* write VALUE:=15 *)
+                             ; (true,  (false, (  4%N, (111%N, tt)))) (* read STATUS *)
+                             ; (true,  (false, (  4%N, (111%N, tt)))) (* read STATUS *)
+                             ; (true,  (false, (  0%N, (111%N, tt)))) (* read VALUE *)
+                           ].
+
+Definition incr_device_step :
+  _ ->
   (* input: current state, is_read_req, is_write_req, req_addr, req_value *)
-  circuit_state incr -> bool * bool * Bvector 32 * Bvector 32 ->
-  (* output: next state, is_resp, resp *)
-  circuit_state incr * (bool * Bvector 32)
+  denote_type [Bit; Bit; BitVec 32; BitVec 32] ->
+  (_
+   (* output: next state, is_resp, resp *)
+   * denote_type (Bit ** BitVec 32))
   := step incr.
 
 Require Import coqutil.Datatypes.List.
 
-(* like `simulate`, but also output the internal state, for more insightful debugging *)
-Fixpoint simulate_with_state_rec{i o}(c: Circuit i o)(initial: circuit_state c)(inps: list i)
-  : list (circuit_state c * o) :=
-  match inps with
-  | [] => []
-  | inp :: rest => let r := step c initial inp in r :: simulate_with_state_rec c (fst r) rest
-  end.
-Definition simulate_with_state{i o}(c: Circuit i o): list i -> list (circuit_state c * o) :=
-  simulate_with_state_rec c (reset_state c).
-
-Example sample_trace := Eval compute in simulate_with_state incr [
-  (false, false, N2Bv_sized 32 111, N2Bv_sized 32 111); (* no action *)
-  (false, true, N2Bv_sized 32 0, N2Bv_sized 32 15);     (* write VALUE:=15 *)
-  (true, false, N2Bv_sized 32 4, N2Bv_sized 32 111);    (* read STATUS *)
-  (true, false, N2Bv_sized 32 4, N2Bv_sized 32 111);    (* read STATUS *)
-  (true, false, N2Bv_sized 32 0, N2Bv_sized 32 111)     (* read VALUE *)
-].
-
-(* Print sample_trace. *)
+(* (* like `simulate`, but also output the internal state, for more insightful debugging *) *)
+(* Fixpoint simulate_with_state_rec {o} *)
+(*          (* (c : Circuit i o) *) *)
+(*          c *)
+(*          (* (initial : circuit_state c) *) *)
+(*          initial *)
+(*          (inps : list type) *)
+(*   (* : list (circuit_state c * o) := *) *)
+(*   := *)
+(*   match inps with *)
+(*   | [] => [] *)
+(*   | inp :: rest => let r := step c initial (denote_type inp) in *)
+(*                  r :: simulate_with_state_rec c (fst r) rest *)
+(*   end *)
+(* . *)
+(* Definition simulate_with_state{i o}(c: Circuit i o): list i -> list (circuit_state c * o) := *)
+(*   simulate_with_state_rec c (reset_state c). *)
 
 Require Import Coq.ZArith.ZArith. Open Scope Z_scope.
 Require Import riscv.Utility.Utility.
@@ -104,12 +119,15 @@ Require Import Bedrock2Experiments.IncrementWait.IncrementWaitSemantics.
 Require Import Bedrock2Experiments.StateMachineSemantics.
 Require Import Bedrock2Experiments.RiscvMachineWithCavaDevice.MMIOToCava.
 
+
+
 Section WithParameters.
+  Context {var : tvar}.
   Context {word: Interface.word 32} {word_ok: word.ok word}
           {Mem: map.map word byte} {Registers: map.map Z word}.
 
-  Definition mk_counter_state(idle busy done: bool)(val: Bvector 32): circuit_state incr :=
-    (tt, (tt, (tt, (tt, (tt, val), done), busy), idle)).
+  Definition mk_counter_state(idle busy done : bool)(val : N) : circuit_state incr :=
+    (idle, (busy, (done, val))).
 
   Global Instance counter_device: device := {|
     device.state := circuit_state incr;
@@ -133,181 +151,182 @@ Section WithParameters.
       counter_related IDLE (mk_counter_state idle false false val)
   | BUSY_related: forall val ncycles,
       (0 < ncycles)%nat ->
-      counter_related (BUSY val ncycles) (mk_counter_state false true false (word_to_bv val))
+      counter_related (BUSY val ncycles) (mk_counter_state false true false (word_to_N val))
   (* the hardware is already done, but the software hasn't polled it yet to find out,
      so we have to relate a software-BUSY to a hardware-done: *)
   | BUSY_done_related: forall val ncycles,
       counter_related (BUSY val ncycles)
-                      (mk_counter_state false false true (word_to_bv (word.add (word.of_Z 1) val)))
+                      (mk_counter_state false false true (word_to_N (word.add (word.of_Z 1) val)))
   | DONE_related: forall val,
-      counter_related (DONE val) (mk_counter_state false false true (word_to_bv val)).
+      counter_related (DONE val) (mk_counter_state false false true (word_to_N val)).
 
-  Axiom TODO: False.
+  Axiom TODO: Coq.Init.Logic.False.
 
-  Axiom word_to_bv_inj: forall x y, word_to_bv x = word_to_bv y -> x = y.
+  Axiom word_to_N_inj: forall x y, word_to_N x = word_to_N y -> x = y.
 
-  Axiom incrN_word_to_bv: forall v, incrN (word_to_bv v) = word_to_bv (word.add (word.of_Z 1) v).
+  Axiom incrN_word_to_bv: forall v, N.add (word_to_N v) 1 = word_to_N (word.add (word.of_Z 1) v).
 
   Set Printing Depth 100000.
 
   Global Instance cava_counter_satisfies_state_machine:
     device_implements_state_machine counter_device increment_wait_state_machine.
   Proof.
-    eapply Build_device_implements_state_machine with (device_state_related := counter_related);
-      intros.
-    - (* mmioAddrs_match: *)
-      reflexivity.
-    - (* initial_state_is_ready_state: *)
-      simpl in *. subst. inversion H0. eauto.
-    - (* initial_states_are_related: *)
-      simpl in *. destruct H0 as (val & idle & H0). subst. eapply IDLE_related.
-    - (* initial_state_exists: *)
-      simpl in *. destruct H as (val & idle & H). subst. eauto using IDLE_related.
-    - (* nonMMIO_device_step_preserves_state_machine_state: *)
-      simpl in sL1, sL2. destruct_state sL1. destruct_state sL2.
-      cbn [device.run1 counter_device incr_device_step step incr incr_update Loop snd
-           ret bind monad CombinationalSemantics Identity.Monad_ident constant] in H0.
-      eapply pair_equal_spec in H0. destruct H0 as [E1 E2].
-      subst.
-      eapply pair_equal_spec in E1. destruct E1 as [_ E1].
-      eapply pair_equal_spec in E1. destruct E1 as [E1 E2]. simpl in E2. subst.
-      eapply pair_equal_spec in E1. destruct E1 as [_ E1].
-      eapply pair_equal_spec in E1. destruct E1 as [E1 E2]. simpl in E2. subst.
-      eapply pair_equal_spec in E1. destruct E1 as [_ E1].
-      eapply pair_equal_spec in E1. destruct E1 as [E1 E2]. simpl in E2. subst.
-      eapply pair_equal_spec in E1. destruct E1 as [_ E1].
-      eapply pair_equal_spec in E1. destruct E1 as [_ E1]. simpl in E1. subst.
-      inversion H; subst.
-      + (* IDLE_related: *)
-        cbn. rewrite andb_false_r. destruct idle; cbn; simpl; eapply IDLE_related.
-      + (* BUSY_related: *)
-        rewrite andb_false_r. cbn -[incrN]. change (Pos.to_nat 1) with 1%nat.
-        cbn -[incrN]. rewrite incrN_word_to_bv.
-        eapply BUSY_done_related.
-      + (* BUSY_done_related: *)
-        cbn. rewrite andb_false_r. cbn. assumption.
-      + (* DONE_related: *)
-        cbn. rewrite andb_false_r. cbn. assumption.
-    - (* state_machine_read_to_device_read: *)
-      (* simpler because device.maxRespDelay=1 *)
-      unfold device.maxRespDelay, device.runUntilResp, device.state, device.run1, counter_device.
-      unfold state_machine.read_step, increment_wait_state_machine in *.
-      simp.
-      unfold read_step in *.
-      destruct r.
-      + (* r=VALUE *)
-        simp.
-        cbn. rewrite andb_false_r. simpl.
-        unfold word_to_bv. rewrite word.unsigned_of_Z_nowrap by (cbv; intuition discriminate).
-        simpl. do 3 eexists. ssplit; try reflexivity. eapply IDLE_related.
-      + (* r=STATUS *)
-        destruct sH.
-        * (* sH=IDLE *)
-          destruct Hp1. subst. inversion H0. subst.
-          cbn. rewrite andb_false_r. simpl. unfold status_value, STATUS_IDLE.
-          unfold word_to_bv.
-          rewrite word.unsigned_of_Z_nowrap by (cbv; intuition discriminate).
-          do 3 eexists. ssplit; try reflexivity. 2: eapply IDLE_related.
-          rewrite word.unsigned_slu. 2: rewrite word.unsigned_of_Z. 2: reflexivity.
-          rewrite !word.unsigned_of_Z. unfold word.wrap. cbn.
-          destruct idle; reflexivity.
-        * (* sH=BUSY *)
-          simp.
-          destruct Hp1 as [H | H].
-          -- (* transition to DONE *)
-             destruct H; subst.
-             simpl (state_machine.reg_addr _).
-             unfold STATUS_ADDR, INCR_BASE_ADDR, word_to_bv, status_value, STATUS_DONE.
-             rewrite !word.unsigned_of_Z. unfold word.wrap. simpl.
-             inversion H0; subst.
-             ++ (* BUSY_related *)
-                (* the transition that was used to show that sH is not stuck was a transition
-                   from BUSY to DONE returning a done flag, but since the device is still
-                   in BUSY state, it will still return the busy flag in this transition,
-                   so the transition we use to simulate what happened in the device is a
-                   BUSY-to-DONE transition returning a busy flag instead of a done flag *)
-                destruct max_cycles_until_done. 1: inversion H3. clear H3.
-                exists (word.of_Z 2). (* <- bit #1 (busy) is set, all others are 0 *)
-                do 2 eexists.
-                rewrite !word.unsigned_of_Z. unfold word.wrap. cbn -[incrN].
-                ssplit; try reflexivity.
-                ** simpl. rewrite incrN_word_to_bv. eapply BUSY_done_related.
-                ** right. eexists; ssplit; try reflexivity. eapply word.unsigned_inj.
-                   rewrite word.unsigned_slu. 2: rewrite word.unsigned_of_Z. 2: reflexivity.
-                   rewrite !word.unsigned_of_Z. reflexivity.
-             ++ (* BUSY_done_related *)
-                exists (word.of_Z 4). (* <- bit #2 (done) is set, all others are 0 *)
-                do 2 eexists.
-                rewrite !word.unsigned_of_Z. unfold word.wrap. cbn -[incrN].
-                ssplit; try reflexivity.
-                ** simpl. eapply DONE_related.
-                ** left. split. 2: reflexivity. eapply word.unsigned_inj.
-                   rewrite word.unsigned_slu. 2: rewrite word.unsigned_of_Z. 2: reflexivity.
-                   rewrite !word.unsigned_of_Z. reflexivity.
-          -- (* stay BUSY *)
-             destruct H as (n & ? & ? & ?); subst.
-             simpl (state_machine.reg_addr _).
-             unfold STATUS_ADDR, INCR_BASE_ADDR, word_to_bv, status_value, STATUS_BUSY.
-             rewrite !word.unsigned_of_Z. unfold word.wrap. simpl.
-             inversion H0; subst.
-             ++ (* BUSY_related *)
-                exists (word.of_Z 2). (* <- bit #1 (busy) is set, all others are 0 *)
-                do 2 eexists.
-                rewrite !word.unsigned_of_Z. unfold word.wrap. cbn -[incrN].
-                ssplit; try reflexivity.
-                ** simpl. rewrite incrN_word_to_bv. eapply BUSY_done_related.
-                ** right. eexists; ssplit; try reflexivity. eapply word.unsigned_inj.
-                   rewrite word.unsigned_slu. 2: rewrite word.unsigned_of_Z. 2: reflexivity.
-                   rewrite !word.unsigned_of_Z. reflexivity.
-             ++ (* BUSY_done_related *)
-                (* the transition that was used to show that sH is not stuck was a transition
-                   from BUSY to BUSY returning a busy flag, but since the device already is
-                   in done state, it will return a done flag in this transition,
-                   so the transition we use to simulate what happened in the device is a
-                   BUSY-to-DONE transition returning a done flag instead of a
-                   BUSY-to-BUSY transition returning a busy flag. *)
-                exists (word.of_Z 4). (* <- bit #2 (done) is set, all others are 0 *)
-                do 2 eexists.
-                rewrite !word.unsigned_of_Z. unfold word.wrap. cbn -[incrN].
-                ssplit; try reflexivity.
-                ** simpl. eapply DONE_related.
-                ** left. split. 2: reflexivity. eapply word.unsigned_inj.
-                   rewrite word.unsigned_slu. 2: rewrite word.unsigned_of_Z. 2: reflexivity.
-                   rewrite !word.unsigned_of_Z. reflexivity.
-        * (* sH=DONE *)
-          destruct Hp1. subst. inversion H0. subst.
-          simpl (state_machine.reg_addr _).
-          unfold STATUS_ADDR, INCR_BASE_ADDR, word_to_bv, status_value, STATUS_DONE.
-          cbn.
-          rewrite !word.unsigned_of_Z. unfold word.wrap. cbn -[Vec.hd Vec.tl incrN].
-          exists (word.of_Z 4). (* <- bit #2 (done) is set, all others are 0 *)
-          do 2 eexists.
-          rewrite !word.unsigned_of_Z. unfold word.wrap. cbn.
-          ssplit; try reflexivity.
-          ** simpl. eapply DONE_related.
-          ** eapply word.unsigned_inj.
-             rewrite word.unsigned_slu. 2: rewrite word.unsigned_of_Z. 2: reflexivity.
-             rewrite !word.unsigned_of_Z. reflexivity.
-    - (* state_machine_write_to_device_write: *)
-      destruct H as (sH' & ? & ?). subst.
-      unfold write_step in H1.
-      destruct r. 2: contradiction.
-      destruct sH; try contradiction. subst.
-      inversion H0. subst.
-      cbn.
-      unfold word_to_bv.
-      rewrite word.unsigned_of_Z_nowrap by (cbv; intuition discriminate).
-      cbn.
-      eexists _, _, _. ssplit; try reflexivity. destruct idle; eapply BUSY_related; lia.
-    - (* read_step_unique: *)
-      cbn in *. unfold read_step in *. simp.
-      destruct v; destruct r; try contradiction; simp; try reflexivity.
-      destruct Hp1; destruct H0p1; simp; try reflexivity;
-        unfold status_value in *; exfalso; ZnWords.
-    - (* write_step_unique: *)
-      cbn in *. unfold write_step in *. simp. subst. reflexivity.
-    - (* initial_state_unique: *)
-      cbn in *. subst. reflexivity.
-  Qed.
+    Admitted.
+    (* eapply Build_device_implements_state_machine with (device_state_related := counter_related); *)
+    (*   intros. *)
+    (* - (* mmioAddrs_match: *) *)
+    (*   reflexivity. *)
+    (* - (* initial_state_is_ready_state: *) *)
+    (*   simpl in *. subst. inversion H0. eauto. *)
+    (* - (* initial_states_are_related: *) *)
+    (*   simpl in *. destruct H0 as (val & idle & H0). subst. eapply IDLE_related. *)
+    (* - (* initial_state_exists: *) *)
+    (*   simpl in *. destruct H as (val & idle & H). subst. eauto using IDLE_related. *)
+    (* - (* nonMMIO_device_step_preserves_state_machine_state: *) *)
+    (*   simpl in sL1, sL2. destruct_state sL1. destruct_state sL2. *)
+    (*   cbn [device.run1 counter_device incr_device_step step incr incr_update Loop snd *)
+    (*        ret bind monad CombinationalSemantics Identity.Monad_ident constant] in H0. *)
+    (*   eapply pair_equal_spec in H0. destruct H0 as [E1 E2]. *)
+    (*   subst. *)
+    (*   eapply pair_equal_spec in E1. destruct E1 as [_ E1]. *)
+    (*   eapply pair_equal_spec in E1. destruct E1 as [E1 E2]. simpl in E2. subst. *)
+    (*   eapply pair_equal_spec in E1. destruct E1 as [_ E1]. *)
+    (*   eapply pair_equal_spec in E1. destruct E1 as [E1 E2]. simpl in E2. subst. *)
+    (*   eapply pair_equal_spec in E1. destruct E1 as [_ E1]. *)
+    (*   eapply pair_equal_spec in E1. destruct E1 as [E1 E2]. simpl in E2. subst. *)
+    (*   eapply pair_equal_spec in E1. destruct E1 as [_ E1]. *)
+    (*   eapply pair_equal_spec in E1. destruct E1 as [_ E1]. simpl in E1. subst. *)
+    (*   inversion H; subst. *)
+    (*   + (* IDLE_related: *) *)
+    (*     cbn. rewrite andb_false_r. destruct idle; cbn; simpl; eapply IDLE_related. *)
+    (*   + (* BUSY_related: *) *)
+    (*     rewrite andb_false_r. cbn -[incrN]. change (Pos.to_nat 1) with 1%nat. *)
+    (*     cbn -[incrN]. rewrite incrN_word_to_bv. *)
+    (*     eapply BUSY_done_related. *)
+    (*   + (* BUSY_done_related: *) *)
+    (*     cbn. rewrite andb_false_r. cbn. assumption. *)
+    (*   + (* DONE_related: *) *)
+    (*     cbn. rewrite andb_false_r. cbn. assumption. *)
+    (* - (* state_machine_read_to_device_read: *) *)
+    (*   (* simpler because device.maxRespDelay=1 *) *)
+    (*   unfold device.maxRespDelay, device.runUntilResp, device.state, device.run1, counter_device. *)
+    (*   unfold state_machine.read_step, increment_wait_state_machine in *. *)
+    (*   simp. *)
+    (*   unfold read_step in *. *)
+    (*   destruct r. *)
+    (*   + (* r=VALUE *) *)
+    (*     simp. *)
+    (*     cbn. rewrite andb_false_r. simpl. *)
+    (*     unfold word_to_bv. rewrite word.unsigned_of_Z_nowrap by (cbv; intuition discriminate). *)
+    (*     simpl. do 3 eexists. ssplit; try reflexivity. eapply IDLE_related. *)
+    (*   + (* r=STATUS *) *)
+    (*     destruct sH. *)
+    (*     * (* sH=IDLE *) *)
+    (*       destruct Hp1. subst. inversion H0. subst. *)
+    (*       cbn. rewrite andb_false_r. simpl. unfold status_value, STATUS_IDLE. *)
+    (*       unfold word_to_bv. *)
+    (*       rewrite word.unsigned_of_Z_nowrap by (cbv; intuition discriminate). *)
+    (*       do 3 eexists. ssplit; try reflexivity. 2: eapply IDLE_related. *)
+    (*       rewrite word.unsigned_slu. 2: rewrite word.unsigned_of_Z. 2: reflexivity. *)
+    (*       rewrite !word.unsigned_of_Z. unfold word.wrap. cbn. *)
+    (*       destruct idle; reflexivity. *)
+    (*     * (* sH=BUSY *) *)
+    (*       simp. *)
+    (*       destruct Hp1 as [H | H]. *)
+    (*       -- (* transition to DONE *) *)
+    (*          destruct H; subst. *)
+    (*          simpl (state_machine.reg_addr _). *)
+    (*          unfold STATUS_ADDR, INCR_BASE_ADDR, word_to_bv, status_value, STATUS_DONE. *)
+    (*          rewrite !word.unsigned_of_Z. unfold word.wrap. simpl. *)
+    (*          inversion H0; subst. *)
+    (*          ++ (* BUSY_related *) *)
+    (*             (* the transition that was used to show that sH is not stuck was a transition *)
+    (*                from BUSY to DONE returning a done flag, but since the device is still *)
+    (*                in BUSY state, it will still return the busy flag in this transition, *)
+    (*                so the transition we use to simulate what happened in the device is a *)
+    (*                BUSY-to-DONE transition returning a busy flag instead of a done flag *) *)
+    (*             destruct max_cycles_until_done. 1: inversion H3. clear H3. *)
+    (*             exists (word.of_Z 2). (* <- bit #1 (busy) is set, all others are 0 *) *)
+    (*             do 2 eexists. *)
+    (*             rewrite !word.unsigned_of_Z. unfold word.wrap. cbn -[incrN]. *)
+    (*             ssplit; try reflexivity. *)
+    (*             ** simpl. rewrite incrN_word_to_bv. eapply BUSY_done_related. *)
+    (*             ** right. eexists; ssplit; try reflexivity. eapply word.unsigned_inj. *)
+    (*                rewrite word.unsigned_slu. 2: rewrite word.unsigned_of_Z. 2: reflexivity. *)
+    (*                rewrite !word.unsigned_of_Z. reflexivity. *)
+    (*          ++ (* BUSY_done_related *) *)
+    (*             exists (word.of_Z 4). (* <- bit #2 (done) is set, all others are 0 *) *)
+    (*             do 2 eexists. *)
+    (*             rewrite !word.unsigned_of_Z. unfold word.wrap. cbn -[incrN]. *)
+    (*             ssplit; try reflexivity. *)
+    (*             ** simpl. eapply DONE_related. *)
+    (*             ** left. split. 2: reflexivity. eapply word.unsigned_inj. *)
+    (*                rewrite word.unsigned_slu. 2: rewrite word.unsigned_of_Z. 2: reflexivity. *)
+    (*                rewrite !word.unsigned_of_Z. reflexivity. *)
+    (*       -- (* stay BUSY *) *)
+    (*          destruct H as (n & ? & ? & ?); subst. *)
+    (*          simpl (state_machine.reg_addr _). *)
+    (*          unfold STATUS_ADDR, INCR_BASE_ADDR, word_to_bv, status_value, STATUS_BUSY. *)
+    (*          rewrite !word.unsigned_of_Z. unfold word.wrap. simpl. *)
+    (*          inversion H0; subst. *)
+    (*          ++ (* BUSY_related *) *)
+    (*             exists (word.of_Z 2). (* <- bit #1 (busy) is set, all others are 0 *) *)
+    (*             do 2 eexists. *)
+    (*             rewrite !word.unsigned_of_Z. unfold word.wrap. cbn -[incrN]. *)
+    (*             ssplit; try reflexivity. *)
+    (*             ** simpl. rewrite incrN_word_to_bv. eapply BUSY_done_related. *)
+    (*             ** right. eexists; ssplit; try reflexivity. eapply word.unsigned_inj. *)
+    (*                rewrite word.unsigned_slu. 2: rewrite word.unsigned_of_Z. 2: reflexivity. *)
+    (*                rewrite !word.unsigned_of_Z. reflexivity. *)
+    (*          ++ (* BUSY_done_related *) *)
+    (*             (* the transition that was used to show that sH is not stuck was a transition *)
+    (*                from BUSY to BUSY returning a busy flag, but since the device already is *)
+    (*                in done state, it will return a done flag in this transition, *)
+    (*                so the transition we use to simulate what happened in the device is a *)
+    (*                BUSY-to-DONE transition returning a done flag instead of a *)
+    (*                BUSY-to-BUSY transition returning a busy flag. *) *)
+    (*             exists (word.of_Z 4). (* <- bit #2 (done) is set, all others are 0 *) *)
+    (*             do 2 eexists. *)
+    (*             rewrite !word.unsigned_of_Z. unfold word.wrap. cbn -[incrN]. *)
+    (*             ssplit; try reflexivity. *)
+    (*             ** simpl. eapply DONE_related. *)
+    (*             ** left. split. 2: reflexivity. eapply word.unsigned_inj. *)
+    (*                rewrite word.unsigned_slu. 2: rewrite word.unsigned_of_Z. 2: reflexivity. *)
+    (*                rewrite !word.unsigned_of_Z. reflexivity. *)
+    (*     * (* sH=DONE *) *)
+    (*       destruct Hp1. subst. inversion H0. subst. *)
+    (*       simpl (state_machine.reg_addr _). *)
+    (*       unfold STATUS_ADDR, INCR_BASE_ADDR, word_to_bv, status_value, STATUS_DONE. *)
+    (*       cbn. *)
+    (*       rewrite !word.unsigned_of_Z. unfold word.wrap. cbn -[Vec.hd Vec.tl incrN]. *)
+    (*       exists (word.of_Z 4). (* <- bit #2 (done) is set, all others are 0 *) *)
+    (*       do 2 eexists. *)
+    (*       rewrite !word.unsigned_of_Z. unfold word.wrap. cbn. *)
+    (*       ssplit; try reflexivity. *)
+    (*       ** simpl. eapply DONE_related. *)
+    (*       ** eapply word.unsigned_inj. *)
+    (*          rewrite word.unsigned_slu. 2: rewrite word.unsigned_of_Z. 2: reflexivity. *)
+    (*          rewrite !word.unsigned_of_Z. reflexivity. *)
+    (* - (* state_machine_write_to_device_write: *) *)
+    (*   destruct H as (sH' & ? & ?). subst. *)
+    (*   unfold write_step in H1. *)
+    (*   destruct r. 2: contradiction. *)
+    (*   destruct sH; try contradiction. subst. *)
+    (*   inversion H0. subst. *)
+    (*   cbn. *)
+    (*   unfold word_to_bv. *)
+    (*   rewrite word.unsigned_of_Z_nowrap by (cbv; intuition discriminate). *)
+    (*   cbn. *)
+    (*   eexists _, _, _. ssplit; try reflexivity. destruct idle; eapply BUSY_related; lia. *)
+    (* - (* read_step_unique: *) *)
+    (*   cbn in *. unfold read_step in *. simp. *)
+    (*   destruct v; destruct r; try contradiction; simp; try reflexivity. *)
+    (*   destruct Hp1; destruct H0p1; simp; try reflexivity; *)
+    (*     unfold status_value in *; exfalso; ZnWords. *)
+    (* - (* write_step_unique: *) *)
+    (*   cbn in *. unfold write_step in *. simp. subst. reflexivity. *)
+    (* - (* initial_state_unique: *) *)
+    (*   cbn in *. subst. reflexivity. *)
+  (* Qed. *)
 
 End WithParameters.
