firmware/RiscvMachineWithCavaDevice/MMIOToCava.v
@@ -50,7 +50,7 @@ Class device_implements_state_machine{word: word.word 32}{mem: map.map word Byte
   nonMMIO_device_step_preserves_state_machine_state:
     forall sL1 sL2 sH ignored_addr ignored_val ignored_resp,
       device_state_related sH sL1 ->
-      device.run1 sL1 (false, false, ignored_addr, ignored_val) = (sL2, ignored_resp) ->
+      device.run1 sL1 (false, (false, (ignored_addr, ignored_val))) = (sL2, ignored_resp) ->
       device_state_related sH sL2;
 
   (* for each high-level state sH from which n bytes can be read at register r,
@@ -63,8 +63,8 @@ Class device_implements_state_machine{word: word.word 32}{mem: map.map word Byte
       (exists v sH', state_machine.read_step n sH r v sH') ->
       device_state_related sH sL ->
       exists v sL' sH',
-        device.runUntilResp true false (word_to_bv (state_machine.reg_addr r)) (word_to_bv (word.of_Z 0))
-                            device.maxRespDelay sL = (Some (word_to_bv v), sL') /\
+        device.runUntilResp true false (word_to_N (state_machine.reg_addr r)) (word_to_N (word.of_Z 0))
+                            device.maxRespDelay sL = (Some (word_to_N v), sL') /\
         device_state_related sH' sL' /\
         state_machine.read_step n sH r v sH';
 
@@ -77,7 +77,7 @@ Class device_implements_state_machine{word: word.word 32}{mem: map.map word Byte
       (exists sH', state_machine.write_step n sH r v sH') ->
       device_state_related sH sL ->
       exists ignored sL' sH',
-        device.runUntilResp false true (word_to_bv (state_machine.reg_addr r)) (word_to_bv v)
+        device.runUntilResp false true (word_to_N (state_machine.reg_addr r)) (word_to_N v)
                             device.maxRespDelay sL = (Some ignored, sL') /\
         device_state_related sH' sL' /\
         state_machine.write_step n sH r v sH';
@@ -227,9 +227,9 @@ Section WithParams.
       eapply step_unique; eassumption.
   Qed.
 
-  Lemma bv_to_word_word_to_bv: forall v, bv_to_word (word_to_bv v) = v.
+  Lemma bv_to_word_word_to_bv: forall v, N_to_word (word_to_N v) = v.
   Proof.
-    intros. unfold bv_to_word, word_to_bv.
+    intros. unfold N_to_word, word_to_N.
   Admitted.
 
   Lemma execution_read_cons: forall n r (v: HList.tuple Byte.byte n) t s1 s2,
